Cook_Levin/IMP-_To_SAS+/IMP_Minus_To_SAS_Plus_Nat.thy
@@ -15,7 +15,12 @@ bit_length (max (max (max_list_nat (ran_nat I)) r) (max_constant_nat c))"
 
 definition max_input_bits_tail :: "nat \<Rightarrow> nat \<Rightarrow> nat\<Rightarrow> nat" where 
 "max_input_bits_tail c I r =
-bit_length (max (max (max_list_tail (ran_tail I)) r) (max_constant_nat c))"
+bit_length (max (max (max_list_tail (ran_tail I)) r) (max_constant_tail c))"
+
+lemma subtail_max_input_bits:
+"max_input_bits_tail c I r = max_input_bits_nat c I r "
+  using max_constant_tail_def max_input_bits_nat_def max_input_bits_tail_def
+ subtail_max_list subtail_ran by presburger
 
 lemma impm_assignment_simp:"impm_assignment_encode = prod_encode o (\<lambda>(a,b). (vname_encode a,b))"
   apply auto
@@ -70,6 +75,22 @@ definition IMP_Minus_initial_to_IMP_Minus_Minus_nat::" nat
    then if k < n then Suc 0 else 0  
  else (if v = vname_encode ''carry'' then Suc 0 
   else (IMP_Minus_State_To_IMP_Minus_Minus_partial_nat I n guess_range) v))" 
+
+definition IMP_Minus_initial_to_IMP_Minus_Minus_tail::" nat 
+  \<Rightarrow> nat \<Rightarrow> nat \<Rightarrow> nat \<Rightarrow> nat" where
+"IMP_Minus_initial_to_IMP_Minus_Minus_tail I n guess_range v =
+  (let p = var_to_operand_bit_tail v; v' = fst_nat (p-1) ; k = snd_nat (p-1) in if
+    p \<noteq> 0 \<and> v' = encode_char (CHR ''a'') then 
+    if k < n then Suc 0 else 0 else if  p \<noteq> 0 \<and> v' = encode_char (CHR ''b'')
+   then if k < n then Suc 0 else 0  
+ else (if v = vname_encode ''carry'' then Suc 0 
+  else (IMP_Minus_State_To_IMP_Minus_Minus_partial_tail I n guess_range) v))"
+
+lemma subtail_IMP_Minus_initial_to_IMP_Minus_Minus:
+"IMP_Minus_initial_to_IMP_Minus_Minus_tail I n guess_range v = 
+IMP_Minus_initial_to_IMP_Minus_Minus_nat I n guess_range v"
+  using IMP_Minus_initial_to_IMP_Minus_Minus_nat_def IMP_Minus_initial_to_IMP_Minus_Minus_tail_def 
+subtail_IMP_Minus_State_To_IMP_Minus_Minus_partial subtail_var_to_operand_bit by presburger
 
 lemma subnat_IMP_Minus_initial_to_IMP_Minus_Minus:
 "IMP_Minus_initial_to_IMP_Minus_Minus_nat (impm_assignment_list_encode I) n guess_range 
@@ -135,14 +156,52 @@ lemma submap_IMP_Minus_State_To_IMP_Minus_Minus_partial :
   apply(induct I  n guess_range x rule: map_IMP_Minus_State_To_IMP_Minus_Minus_partial.induct)
   apply auto
   done
+fun map_IMP_Minus_State_To_IMP_Minus_Minus_partial_acc :: "nat \<Rightarrow> nat \<Rightarrow> nat \<Rightarrow> nat \<Rightarrow> nat \<Rightarrow> nat" where 
+"map_IMP_Minus_State_To_IMP_Minus_Minus_partial_acc acc I n guess_range x = (if x =0 then acc else  map_IMP_Minus_State_To_IMP_Minus_Minus_partial_acc (
+( prod_encode(hd_nat x,IMP_Minus_State_To_IMP_Minus_Minus_partial_nat I n guess_range (hd_nat x)))## acc) I n guess_range (tl_nat x) )"
 
-fun filter_none :: "nat \<Rightarrow> nat" where 
+lemma map_IMP_Minus_State_To_IMP_Minus_Minus_partial_induct:
+"map_IMP_Minus_State_To_IMP_Minus_Minus_partial_acc acc  I n guess_range x = 
+ map_acc (\<lambda>x. prod_encode(x,IMP_Minus_State_To_IMP_Minus_Minus_partial_nat I n guess_range x)) acc x  "
+  apply(induct acc I n guess_range x rule: map_IMP_Minus_State_To_IMP_Minus_Minus_partial_acc.induct)
+  apply auto
+  done
+
+definition map_IMP_Minus_State_To_IMP_Minus_Minus_partial_tail ::"nat \<Rightarrow> nat \<Rightarrow> nat \<Rightarrow> nat \<Rightarrow> nat" where 
+"map_IMP_Minus_State_To_IMP_Minus_Minus_partial_tail   I n guess_range x =
+reverse_nat (map_IMP_Minus_State_To_IMP_Minus_Minus_partial_acc 0  I n guess_range x)  "
+
+lemma subtail_map_IMP_Minus_State_To_IMP_Minus_Minus_partial:
+"map_IMP_Minus_State_To_IMP_Minus_Minus_partial_tail   I n guess_range x =
+map_IMP_Minus_State_To_IMP_Minus_Minus_partial   I n guess_range x "
+  using IMP_Minus_To_SAS_Plus_Nat.map_IMP_Minus_State_To_IMP_Minus_Minus_partial_induct 
+IMP_Minus_To_SAS_Plus_Nat.map_IMP_Minus_State_To_IMP_Minus_Minus_partial_tail_def
+ IMP_Minus_To_SAS_Plus_Nat.submap_IMP_Minus_State_To_IMP_Minus_Minus_partial 
+subtail_map by presburger
+
+fun filter_none :: "nat \<Rightarrow> nat" where
 "filter_none n = (if n =0 then 0 else if snd_nat (hd_nat n) \<noteq> 0 then (hd_nat n) ## (filter_none (tl_nat n)) else filter_none (tl_nat n))"
+
+fun filter_none_acc :: "nat \<Rightarrow> nat \<Rightarrow> nat" where 
+"filter_none_acc acc n = (if n =0 then acc else if snd_nat (hd_nat n) \<noteq> 0 then filter_none_acc ((hd_nat n) ## acc) (tl_nat n) else filter_none_acc acc (tl_nat n))"
+
 lemma subfilter_none :
 "filter_none n = filter_nat (\<lambda>n . snd_nat n \<noteq> 0) n"
   apply (induct n rule: filter_none.induct)
   apply auto
   done
+lemma filter_none_induct : 
+"filter_none_acc acc n = filter_acc (\<lambda>n . snd_nat n \<noteq> 0) acc n"
+  apply(induct acc n rule:filter_none_acc.induct)
+  apply auto
+  done
+
+definition filter_none_tail :: "nat \<Rightarrow> nat" where 
+"filter_none_tail n = reverse_nat (filter_none_acc 0 n)"
+
+lemma subtail_filter_none:
+"filter_none_tail n = filter_none n"
+  using filter_none_induct filter_none_tail_def subfilter_none subtail_filter by presburger
 
 fun map_prod_the :: "nat \<Rightarrow> nat" where 
 "map_prod_the n = (if n = 0 then 0 else (prod_encode(fst_nat (hd_nat n), the_nat (snd_nat (hd_nat n)))) ## map_prod_the(tl_nat n) )"
@@ -152,6 +211,22 @@ lemma submap_prod_the:
   apply (induct n rule:map_prod_the.induct)
   apply auto
   done
+
+fun map_prod_the_acc :: "nat\<Rightarrow> nat \<Rightarrow> nat" where 
+"map_prod_the_acc acc n = (if n = 0 then acc else map_prod_the_acc ( (prod_encode(fst_nat (hd_nat n), the_nat (snd_nat (hd_nat n)))) ## acc) (tl_nat n) )"
+
+lemma map_prod_the_induct:
+"map_prod_the_acc acc n = map_acc (\<lambda>n. prod_encode(fst_nat n, the_nat (snd_nat n))) acc n "
+  apply(induct acc n rule:map_prod_the_acc.induct)
+  apply auto
+  done
+
+definition map_prod_the_tail :: "nat \<Rightarrow> nat" where 
+"map_prod_the_tail n = reverse_nat (map_prod_the_acc 0 n)"
+
+lemma subtail_map_prod_the:
+"map_prod_the_tail n = map_prod_the n"
+  using map_prod_the_induct map_prod_the_tail_def submap_prod_the subtail_map by presburger
 
 definition IMP_Minus_to_SAS_Plus_nat:: "nat \<Rightarrow> nat \<Rightarrow> nat \<Rightarrow> nat
   \<Rightarrow>  nat \<Rightarrow> nat" where
@@ -168,6 +243,27 @@ map_prod_the (filter_none (map_IMP_Minus_State_To_IMP_Minus_Minus_partial I n gu
   SAS_Plus_Plus_To_SAS_Plus_nat (imp_minus_minus_to_sas_plus_nat c' I' G'))"
 
 
+definition IMP_Minus_to_SAS_Plus_tail:: "nat \<Rightarrow> nat \<Rightarrow> nat \<Rightarrow> nat
+  \<Rightarrow>  nat \<Rightarrow> nat" where
+"IMP_Minus_to_SAS_Plus_tail c I r G t = (let 
+  guess_range = max_input_bits_tail c I r;
+  n = t + guess_range + 1;
+  c' = IMP_Minus_To_IMP_Minus_Minus_tail c n;
+  I' = 
+map_prod_the_tail (filter_none_tail (map_IMP_Minus_State_To_IMP_Minus_Minus_partial_tail I n guess_range (enumerate_variables_tail c')))
+;
+
+  G' = map_prod_the_tail (filter_none_tail (map_IMP_Minus_State_To_IMP_Minus_Minus_partial_tail G n n (enumerate_variables_tail c')))
+ in
+  SAS_Plus_Plus_To_SAS_Plus_tail (imp_minus_minus_to_sas_plus_tail c' I' G'))"
+
+lemma subtail_IMP_Minus_to_SAS_Plus:
+"IMP_Minus_to_SAS_Plus_tail c I r G t = IMP_Minus_to_SAS_Plus_nat c I r G t "
+  using IMP_Minus_To_IMP_Minus_Minus_tail_def
+ IMP_Minus_To_SAS_Plus_Nat.subtail_map_IMP_Minus_State_To_IMP_Minus_Minus_partial 
+IMP_Minus_to_SAS_Plus_nat_def IMP_Minus_to_SAS_Plus_tail_def subtail_SAS_Plus_Plus_To_SAS_Plus 
+subtail_enumerate_variables subtail_filter_none subtail_imp_minus_minus_to_sas_plus
+ subtail_map_prod_the subtail_max_input_bits by presburger
 
 lemma thef_bit_option_lambda:"
 map (\<lambda>x. prod_encode
