Cook_Levin/IMP-_To_SAS+/IMP_Minus_To_SAT_Nat.thy
@@ -49,6 +49,9 @@ qed
 fun poly_of_nat :: "nat \<Rightarrow> nat \<Rightarrow> nat" where 
 "poly_of_nat p x = (if snd_nat p = 0 then fst_nat p else x * poly_of_nat (prod_encode (fst_nat p,snd_nat p -1)) x)"
 
+fun poly_of_acc :: "nat \<Rightarrow> nat \<Rightarrow> nat \<Rightarrow> nat" where 
+"poly_of_acc acc p x = (if snd_nat p = 0 then acc else poly_of_acc  (x *acc) (prod_encode (fst_nat p,snd_nat p -1)) x)"
+
 lemma sub_poly_of: "poly_of_nat (prod_encode p) x = poly_of p x"
   apply (cases p)
   apply (auto simp only:)
@@ -61,8 +64,43 @@ lemma sub_poly_of: "poly_of_nat (prod_encode p) x = poly_of p x"
     done
   done
 
+
+lemma poly_of_induct:
+"poly_of_acc acc p x = poly_of_nat (prod_encode (acc,snd_nat p)) x"
+proof -
+
+  obtain a n where p_def:"p = prod_encode (a,n)"
+    by (metis prod_decode_inverse surj_pair)
+   have helper:"\<forall>m acc. poly_of (x * acc,m) x = x * poly_of (acc,m) x"
+     apply auto subgoal for m acc
+        apply(induct m) apply auto done done
+   from p_def show ?thesis apply(auto simp only: sub_snd snd_conv sub_poly_of)
+    apply (induct n arbitrary: p  acc a)
+     apply(subst poly_of_acc.simps)
+     apply(auto simp add: sub_snd simp del: poly_of_acc.simps)
+     apply(subst poly_of_acc.simps)
+    apply(auto simp add: helper sub_fst sub_snd simp del: poly_of_acc.simps)
+     done
+    
+qed
+
+definition poly_of_tail :: "nat \<Rightarrow> nat \<Rightarrow> nat" where 
+"poly_of_tail p x = poly_of_acc (fst_nat p) p x"
+
+lemma subtail_poly_of:
+"poly_of_tail p x = poly_of_nat p x"
+  by (metis add.right_neutral add_eq_if poly_of.simps(1)
+ poly_of.simps(2) poly_of_induct poly_of_nat.simps poly_of_tail_def sub_poly_of)
+
 definition t'_nat :: "nat \<Rightarrow> nat \<Rightarrow> nat \<Rightarrow> nat" where 
 "t'_nat pt p_cer x = poly_of_nat pt (bit_length x + poly_of_nat p_cer (bit_length x)) + 1"
+
+definition t'_tail :: "nat \<Rightarrow> nat \<Rightarrow> nat \<Rightarrow> nat" where 
+"t'_tail pt p_cer x = poly_of_tail pt (bit_length x + poly_of_tail p_cer (bit_length x)) + 1"
+
+lemma subtail_t':
+"t'_tail pt p_cer x = t'_nat pt p_cer x"
+  using subtail_poly_of t'_nat_def t'_tail_def by presburger
 
 lemma subnat_t': 
 "t'_nat (prod_encode pt) (prod_encode p_cer) x = t'_pair pt p_cer x"
@@ -77,6 +115,11 @@ lemma sub_empty_sasp_action: "empty_sasp_action_nat = operator_plus_encode empty
         simp flip: list_encode.simps)
    apply auto
   done
+definition "empty_sasp_action_tail \<equiv> (0 ## 0 ## 0)"
+lemma subtail_empty_sasp_action:
+"empty_sasp_action_tail =empty_sasp_action_nat"
+  using empty_sasp_action_nat_def empty_sasp_action_tail_def by force
+
 
 definition
   "prob_with_noop_list \<Pi> \<equiv>
@@ -94,6 +137,15 @@ lemma sublist_prob_with_noop:
 definition prob_with_noop_nat :: "nat \<Rightarrow> nat" where 
   "prob_with_noop_nat p = (nth_nat 0 p) ## ( empty_sasp_action_nat ##  (nth_nat (Suc 0) p))
 ## (tl_nat (tl_nat p))"
+
+definition prob_with_noop_tail :: "nat \<Rightarrow> nat" where 
+  "prob_with_noop_tail p = (nth_nat 0 p) ## ( empty_sasp_action_tail ##  (nth_nat (Suc 0) p))
+## (tl_nat (tl_nat p))"
+
+
+lemma subtail_prob_with_noop:
+"prob_with_noop_tail p =prob_with_noop_nat p"
+  using prob_with_noop_nat_def prob_with_noop_tail_def subtail_empty_sasp_action by presburger
 
 lemma subnat_prob_with_noop: 
 "prob_with_noop_nat (list_problem_plus_encode p) = 
@@ -134,6 +186,18 @@ definition encode_interfering_operator_pair_exclusion_nat
     \<equiv> let ops = nth_nat (Suc 0)  p in
      4 ## (2 ## (1 ## (1 ## k ## (index_nat ops o1)## 0) ## 0) ## 0)
       ## (2 ## (1 ## (1  ## k ## (index_nat ops o2) ## 0) ## 0) ## 0) ## 0"
+definition encode_interfering_operator_pair_exclusion_tail :: "nat
+    \<Rightarrow> nat
+    \<Rightarrow> nat
+    \<Rightarrow> nat
+    \<Rightarrow> nat" where 
+"encode_interfering_operator_pair_exclusion_tail p k o1 o2 =
+encode_interfering_operator_pair_exclusion_nat p k o1 o2 "
+
+lemma subtail_encode_interfering_operator_pair_exclusion:
+"encode_interfering_operator_pair_exclusion_tail p k o1 o2 =
+encode_interfering_operator_pair_exclusion_nat p k o1 o2 "
+  using encode_interfering_operator_pair_exclusion_tail_def by presburger
 
 lemma subnat_encode_interfering_operator_pair_exclusion:
 "encode_interfering_operator_pair_exclusion_nat (strips_list_problem_encode p) k
@@ -152,6 +216,14 @@ declare elemof.simps [simp del]
 fun list_inter :: "nat \<Rightarrow> nat \<Rightarrow> nat" where 
 "list_inter xs ys = (if xs = 0 then 0 
 else if elemof (hd_nat xs) ys \<noteq> 0 then 1 else list_inter (tl_nat xs) ys)"
+
+definition list_inter_tail ::  "nat \<Rightarrow> nat \<Rightarrow> nat" where 
+"list_inter_tail xs ys = list_inter xs ys"
+
+lemma subtail_list_inter:
+"list_inter_tail xs ys = list_inter xs ys"
+  using list_inter_tail_def by presburger
+
 
 lemma list_encode_pos:"(list_encode xs > 0) = (xs \<noteq> []) "
   using list_encode_empty by force
@@ -181,6 +253,15 @@ definition are_operators_interfering_nat :: "nat \<Rightarrow> nat \<Rightarrow>
 "are_operators_interfering_nat o1 o2 \<equiv>
 if list_inter (nth_nat (Suc (Suc 0)) o1) (nth_nat 0 o2) \<noteq> 0  \<or> 
     list_inter (nth_nat 0 o1) (nth_nat (Suc (Suc 0)) o2) \<noteq> 0 then 1 else 0 "
+
+definition are_operators_interfering_tail :: "nat \<Rightarrow> nat \<Rightarrow> nat" where
+"are_operators_interfering_tail o1 o2 \<equiv>
+if list_inter_tail (nth_nat (Suc (Suc 0)) o1) (nth_nat 0 o2) \<noteq> 0  \<or> 
+    list_inter_tail (nth_nat 0 o1) (nth_nat (Suc (Suc 0)) o2) \<noteq> 0 then 1 else 0 "
+lemma subtail_are_operators_interfering:
+"are_operators_interfering_tail o1 o2 = are_operators_interfering_nat o1 o2"
+  using are_operators_interfering_nat_def are_operators_interfering_tail_def 
+list_inter_tail_def by presburger
 
 lemma sub_are_operators_interfering:
 "(are_operators_interfering_nat (strips_operator_encode o1) (strips_operator_encode o2) > 0) =
@@ -215,12 +296,33 @@ fun filter_interfering:: "nat \<Rightarrow> nat \<Rightarrow> nat" where
 "filter_interfering ops xs = (if xs = 0 then 0 else if index_nat ops (fst_nat (hd_nat xs)) \<noteq> index_nat ops (snd_nat (hd_nat xs))
         \<and> are_operators_interfering_nat (fst_nat (hd_nat xs)) (snd_nat (hd_nat xs)) \<noteq> 0 then (hd_nat xs) ## filter_interfering ops (tl_nat xs) else  filter_interfering ops (tl_nat xs))"
 
+fun filter_interfering_acc:: "nat \<Rightarrow> nat \<Rightarrow> nat \<Rightarrow> nat" where 
+"filter_interfering_acc acc ops xs = (if xs = 0 then acc else if index_nat ops (fst_nat (hd_nat xs)) \<noteq> index_nat ops (snd_nat (hd_nat xs))
+        \<and> are_operators_interfering_tail (fst_nat (hd_nat xs)) (snd_nat (hd_nat xs)) \<noteq> 0 then filter_interfering_acc ((hd_nat xs) ## acc) ops (tl_nat xs) else  filter_interfering_acc acc ops (tl_nat xs))"
+
+lemma filter_interfering_induct:
+"filter_interfering_acc acc ops xs  = filter_acc  (\<lambda>n. index_nat ops (fst_nat n) \<noteq> index_nat ops (snd_nat n)
+        \<and> are_operators_interfering_nat (fst_nat n) (snd_nat n) \<noteq> 0 ) acc xs "
+  apply(induct acc ops xs rule:filter_interfering_acc.induct)
+  apply (auto simp add:subtail_are_operators_interfering)
+  done
+
+
 lemma subfilter_interfering:
 "filter_interfering ops xs = filter_nat (\<lambda>n. index_nat ops (fst_nat n) \<noteq> index_nat ops (snd_nat n)
         \<and> are_operators_interfering_nat (fst_nat n) (snd_nat n) \<noteq> 0 ) xs"
   apply (induct ops xs rule:filter_interfering.induct)
   apply (auto simp del:index_nat.simps)
   done
+
+definition filter_interfering_tail :: "nat \<Rightarrow> nat \<Rightarrow> nat" where
+"filter_interfering_tail ops xs = reverse_nat (filter_interfering_acc 0 ops xs )  "
+
+lemma subtail_filter_interfering:
+"filter_interfering_tail ops xs = filter_interfering ops xs "
+  using filter_interfering_induct filter_interfering_tail_def subfilter_interfering subtail_filter
+  by presburger
+
 fun map_encode_interfering :: "nat \<Rightarrow> nat \<Rightarrow> nat \<Rightarrow> nat" where 
 "map_encode_interfering p n xs = (if xs = 0 then 0 else (encode_interfering_operator_pair_exclusion_nat p (hd_nat xs) (fst_nat n) (snd_nat n)) 
 ## map_encode_interfering p n (tl_nat xs))"
@@ -229,11 +331,36 @@ lemma submap_encode_interfering:
   apply (induct p n xs rule: map_encode_interfering.induct)
   apply auto
   done
+fun map_encode_interfering_acc :: "nat \<Rightarrow> nat \<Rightarrow> nat \<Rightarrow> nat \<Rightarrow> nat" where 
+"map_encode_interfering_acc acc  p n xs = (if xs = 0 then acc else
+map_encode_interfering_acc ((encode_interfering_operator_pair_exclusion_nat p (hd_nat xs) (fst_nat n) (snd_nat n)) 
+## acc) p n (tl_nat xs))"
+
+lemma map_encode_interfering_induct:
+"map_encode_interfering_acc acc  p n xs = map_acc
+(\<lambda>k. encode_interfering_operator_pair_exclusion_tail p k (fst_nat n) (snd_nat n)) acc xs"
+  apply(induct acc p n xs rule:map_encode_interfering_acc.induct)
+  apply (auto simp add:subtail_encode_interfering_operator_pair_exclusion)
+  done
+
 
 fun map_map_encode_interfering :: "nat \<Rightarrow>nat \<Rightarrow> nat \<Rightarrow> nat" where 
 "map_map_encode_interfering \<Pi> t xs = (if xs = 0 then 0 else 
 (map_encode_interfering  \<Pi> (hd_nat xs) (list_less_nat t)) ## map_map_encode_interfering \<Pi> t (tl_nat xs) 
 ) "
+
+fun map_map_encode_interfering_acc :: "nat \<Rightarrow> nat \<Rightarrow>nat \<Rightarrow> nat \<Rightarrow> nat" where 
+"map_map_encode_interfering_acc acc \<Pi> t xs = (if xs = 0 then acc else  map_map_encode_interfering_acc(
+(map_encode_interfering  \<Pi> (hd_nat xs) (list_less_nat t)) ## acc) \<Pi> t (tl_nat xs) 
+) "
+
+lemma map_map_encode_interfering_induct:
+"map_map_encode_interfering_acc acc \<Pi> t xs = map_acc (\<lambda>n. map_encode_interfering  \<Pi> n
+      (list_less_nat t) ) acc xs "
+  apply(induct acc \<Pi> t xs rule: map_map_encode_interfering_acc.induct)
+  apply auto
+  done
+
 lemma submap_map_encode_interfering:
 "map_map_encode_interfering \<Pi> t xs = map_nat (\<lambda>n. map_encode_interfering  \<Pi> n
       (list_less_nat t) ) xs "
@@ -241,12 +368,34 @@ lemma submap_map_encode_interfering:
   apply auto
   done
 
+definition map_map_encode_interfering_tail :: "nat \<Rightarrow> nat \<Rightarrow> nat \<Rightarrow> nat" where 
+"map_map_encode_interfering_tail \<Pi> t xs = reverse_nat (map_map_encode_interfering_acc 0 \<Pi> t xs)"
+
+lemma subtail_map_map_encode_interfering:
+"map_map_encode_interfering_tail \<Pi> t xs = map_map_encode_interfering \<Pi> t xs "
+  using map_map_encode_interfering_induct map_map_encode_interfering_tail_def
+ submap_map_encode_interfering subtail_map by presburger
+
 definition encode_interfering_operator_exclusion_nat
   :: "nat \<Rightarrow> nat \<Rightarrow> nat"
   where "encode_interfering_operator_exclusion_nat \<Pi> t \<equiv> let
       ops = nth_nat (Suc 0) \<Pi>
       ; interfering = filter_interfering ops (product_nat ops ops)
     in BigAnd_nat (concat_nat (map_map_encode_interfering \<Pi> t interfering ))"
+
+definition encode_interfering_operator_exclusion_tail
+  :: "nat \<Rightarrow> nat \<Rightarrow> nat"
+  where "encode_interfering_operator_exclusion_tail \<Pi> t \<equiv> let
+      ops = nth_nat (Suc 0) \<Pi>
+      ; interfering = filter_interfering_tail ops (product_tail ops ops)
+    in BigAnd_tail (concat_tail (map_map_encode_interfering_tail \<Pi> t interfering ))"
+
+lemma subtail_encode_interfering_operator_exclusion:
+"encode_interfering_operator_exclusion_tail p t = encode_interfering_operator_exclusion_nat p t "
+  using encode_interfering_operator_exclusion_nat_def encode_interfering_operator_exclusion_tail_def
+ subtail_BigAnd subtail_concat subtail_filter_interfering subtail_map_map_encode_interfering 
+subtail_product by presburger
+
 lemma subnat_encode_interfering_operator_exclusion :
 "encode_interfering_operator_exclusion_nat (strips_list_problem_encode p) t =
 sat_formula_encode (encode_interfering_operator_exclusion_list p t)"
@@ -293,6 +442,23 @@ definition encode_problem_with_operator_interference_exclusion_nat
       ## (3 ## (encode_all_frame_axioms_nat \<Pi> t)
       ## (3 ## (encode_interfering_operator_exclusion_nat \<Pi> t)
       ## (encode_goal_state_nat \<Pi> t) ## 0) ## 0 )## 0) ## 0"
+
+definition encode_problem_with_operator_interference_exclusion_tail
+  :: "nat\<Rightarrow> nat \<Rightarrow> nat"
+  where "encode_problem_with_operator_interference_exclusion_tail \<Pi> t
+    \<equiv> 3 ## (encode_initial_state_tail \<Pi>)
+      ## (3 ## (encode_operators_tail \<Pi> t)
+      ## (3 ## (encode_all_frame_axioms_tail \<Pi> t)
+      ## (3 ## (encode_interfering_operator_exclusion_tail \<Pi> t)
+      ## (encode_goal_state_tail \<Pi> t) ## 0) ## 0 )## 0) ## 0"
+
+lemma subtail_encode_problem_with_operator_interference_exclusion:
+"encode_problem_with_operator_interference_exclusion_tail \<Pi> t =
+ encode_problem_with_operator_interference_exclusion_nat \<Pi> t"
+  using encode_problem_with_operator_interference_exclusion_nat_def
+ encode_problem_with_operator_interference_exclusion_tail_def subtail_encode_all_frame_axioms
+ subtail_encode_goal_state subtail_encode_initial_state subtail_encode_interfering_operator_exclusion 
+subtail_encode_operators by presburger
 
 lemma subnat_encode_problem_with_operator_interference_exclusion:
 "encode_problem_with_operator_interference_exclusion_nat (strips_list_problem_encode \<Pi>) t =
@@ -395,6 +561,28 @@ lemma main_lemma_hol_list:
         (sas_plus_problem_to_strips_problem_nat (prob_with_noop_nat (IMP_Minus_to_SAS_Plus_nat c I guess_range G (t'_nat pt p_cer x))))
            (100 * (max_bits + (t'_nat pt p_cer x) + 1) * ((t'_nat pt p_cer x) - 1) +
              (max_bits + (t'_nat pt p_cer x) + 2) * (num_variables_nat c + 2) + 52))"
+
+definition imp_to_sat_tail :: "nat \<Rightarrow> nat \<Rightarrow> nat \<Rightarrow> nat \<Rightarrow> nat" where
+    "imp_to_sat_tail c pt p_cer x =
+      (let I = (prod_encode (vname_encode ''input'', x)) ## 0; 
+          G = (prod_encode (vname_encode ''input'', 0)) ## 0;
+          guess_range = x + 1 + 2 * 2 ^ (poly_of_tail p_cer (bit_length x));
+          max_bits = max_input_bits_tail c I guess_range
+      in
+        encode_problem_with_operator_interference_exclusion_tail 
+        (sas_plus_problem_to_strips_problem_tail (prob_with_noop_tail (IMP_Minus_to_SAS_Plus_tail c I guess_range G (t'_tail pt p_cer x))))
+           (100 * (max_bits + (t'_tail pt p_cer x) + 1) * ((t'_tail pt p_cer x) - 1) +
+             (max_bits + (t'_tail pt p_cer x) + 2) * (num_variables_tail c + 2) + 52))"
+
+lemma subtail_imp_to_sat :
+"imp_to_sat_tail c pt p_cer x = imp_to_sat_nat c pt p_cer x"
+  apply(auto simp only: imp_to_sat_tail_def imp_to_sat_nat_def
+subtail_poly_of subtail_max_input_bits subtail_encode_problem_with_operator_interference_exclusion
+subtail_sas_plus_problem_to_strips_problem subtail_prob_with_noop subtail_IMP_Minus_to_SAS_Plus
+subtail_t' subtail_num_variables
+)
+  done
+
 lemma unfold_map_signleton:"[f x] = map f [x]"
   apply auto
   done
@@ -421,18 +609,21 @@ proof -
     by fast
   hence "is_valid_problem_sas_plus (list_problem_to_problem (prob_with_noop_list ?P))"
     using sublist_prob_with_noop by metis
-  thus " encode_problem_with_operator_interference_exclusion_nat
-     (\<phi> list_problem_plus_encode
-          (prob_with_noop_list
-            (IMP_Minus_to_SAS_Plus_list c [(''input'', x)]
-              (x + 1 + 2 * 2 ^ poly_of p_cer (Bit_Length.bit_length x)) [(''input'', 0)]
-              (t'_pair pt p_cer x))) )
+  thus "encode_problem_with_operator_interference_exclusion_nat
+     (sas_plus_problem_to_strips_problem_nat
+       (list_problem_plus_encode
+         (prob_with_noop_list
+           (IMP_Minus_to_SAS_Plus_list c [(''input'', x)]
+             (x + 1 + 2 * 2 ^ poly_of p_cer (Bit_Length.bit_length x)) [(''input'', 0)]
+             (t'_pair pt p_cer x)))))
      (100 *
-      (max_input_bits_list c [(''input'', x)] (x + 1 + 2 * 2 ^ poly_of p_cer (Bit_Length.bit_length x)) +
+      (max_input_bits_list c [(''input'', x)]
+        (x + 1 + 2 * 2 ^ poly_of p_cer (Bit_Length.bit_length x)) +
        t'_pair pt p_cer x +
        1) *
       (t'_pair pt p_cer x - 1) +
-      (max_input_bits_list c [(''input'', x)] (x + 1 + 2 * 2 ^ poly_of p_cer (Bit_Length.bit_length x)) +
+      (max_input_bits_list c [(''input'', x)]
+        (x + 1 + 2 * 2 ^ poly_of p_cer (Bit_Length.bit_length x)) +
        t'_pair pt p_cer x +
        2) *
       (num_variables c + 2) +
@@ -471,5 +662,25 @@ lemma main_lemma_hol_nat:
                    \<and> (Sema.sat {f}  \<longleftrightarrow> in_lang x = 0))"
   using assms main_lemma_hol_list by (auto simp add:subnat_imp_to_sat inj_formula_simp)
 
+lemma main_lemma_hol_tail:
+  fixes c and pt::"nat*nat" and p_cer::"nat*nat" and in_lang
+  assumes verifier_tbounded:
+    "\<And>s. \<exists>t s'. (c, s) \<Rightarrow>\<^bsup> t \<^esup> s' \<and>
+                   t \<le> poly_of pt (bit_length (s ''input''))"
+  assumes verifier_terminates: 
+          "\<And>x s. \<lbrakk>in_lang x = 0 ; s ''input'' = x\<rbrakk> \<Longrightarrow>
+                    (\<exists>z t s'. bit_length z \<le> poly_of p_cer (bit_length x) \<and>
+                              (c, s(''certificate'' := z)) \<Rightarrow>\<^bsup> t \<^esup> s' \<and>
+                              s' ''input'' = in_lang x)"
+          "\<And>x s s' t. \<lbrakk>in_lang x \<noteq> 0; s ''input'' = x; (c, s) \<Rightarrow>\<^bsup> t \<^esup> s'\<rbrakk> \<Longrightarrow>
+                         s' ''input'' = in_lang x"
+  assumes verifier_has_registers:
+    "''input'' \<in> set (Max_Constant.all_variables c)"
+  shows "\<exists>t_red s_red.
+         poly t_red 
+       \<and> poly s_red
+       \<and> (\<forall>x. \<exists>f.  bit_length (encode_sat f) \<le> s_red ( bit_length x ) \<and> imp_to_sat_tail(com_encode c) (prod_encode pt) (prod_encode p_cer) x = sat_formula_encode f
+                   \<and> (Sema.sat {f}  \<longleftrightarrow> in_lang x = 0))"
+  using assms main_lemma_hol_nat by (auto simp add:subtail_imp_to_sat inj_formula_simp)
 
 end
